\documentclass[12pt]{article}
\usepackage[utf8]{inputenc}
\usepackage{listings}
\lstset{
	language=Octave,
	frame=single,
	xleftmargin=.1\textwidth, xrightmargin=.1\textwidth
}
\usepackage{graphicx}
\usepackage{mathtools, nccmath}
\usepackage[T2A]{fontenc}
\usepackage[utf8]{inputenc}
\usepackage[russian]{babel}
\usepackage{amsmath}
\usepackage[left=2cm,right=2cm,top=2cm,bottom=2.1cm,bindingoffset=0cm]{geometry}
\usepackage{amsfonts}
\usepackage{minted}
\usepackage{amssymb}
\usepackage{textcomp}

\graphicspath{{/pic}}
\DeclarePairedDelimiter{\nint}\lfloor\rfloor
\DeclarePairedDelimiter{\hint}\lceil\rceil

\title{Методы оптимизации, лабораторная № 1}

\Large

\begin{document}
	\maketitle
	
\section{Логистическая регрессия}

\subsection{Вычисление ответа}
$$a(x) = sign(\langle\,w,x\rangle)$$

$$p_+(x) = \sigma(\langle\,w,x\rangle)$$

\subsection{Функционал качества}

$$Q(w) = \frac{1}{L}\sum\limits_{i = 1}^L ln(1 + e^{-\langle\,w,x_i\rangle\cdot y_i})$$

$$Q^{l_2}(w) = Q(w) + \frac{\lambda}{2}||w||^2 = Q(w) + \frac{\lambda}{2} \sum\limits_{i = 1}^{F+1}w_i^2$$

\subsection{Градиент}

$$\frac{\partial Q}{\partial w_j} = \frac{1}{L}\sum\limits_{i = 1}^{L}-\frac{e^{-\langle\,w,x_i\rangle\cdot y_i} \cdot y_i \cdot x_{i, j}}{1 + e^{-\langle\,w,x_i\rangle\cdot y_i}} = -\frac{1}{L}\sum\limits_{i = 1}^{L}\frac{y_i \cdot x_{i, j}}{1 + e^{\langle\,w,x_i\rangle\cdot y_i}} $$

\[ 
\left( \frac{\partial Q}{\partial w} \right)_{F+1} =-\frac{1}{L} A_{F+1, L} \cdot b_{L}
\]

$$A_{j, i} = y_{i} \cdot x_{i, j}$$

$$b_i = \frac{1}{1 + e^{\langle\,w,x_i\rangle\cdot y_i}}$$

$$\frac{\partial Q^{l_2}}{\partial w_j} = \frac{\partial Q}{\partial w_j}  + \lambda \cdot w_j $$

$$\frac{\partial Q^{l_2}}{\partial w} = \frac{\partial Q}{\partial w}  + \lambda \cdot w = -\frac{1}{L} A \cdot b + \lambda w$$

\subsection{Гессиан}

$$\frac{\partial^2 Q}{\partial w_j \partial w_k} = \frac{\partial}{\partial w_k} \frac{\partial Q}{\partial w_j} = \frac{1}{L}\sum\limits_{i = 1}^{L} \frac{x_{i, j} \cdot x_{i, k} \cdot y_i^2 \cdot e^{\langle\,w,x_i\rangle \cdot y_i}}{(e^{\langle\,w,x_i\rangle \cdot y_i} + 1)^2} = \frac{1}{L}\sum\limits_{i = 1}^{L} \frac{x_{i, j} \cdot x_{i, k} \cdot e^{\langle\,w,x_i\rangle \cdot y_i}}{(e^{\langle\,w,x_i\rangle \cdot y_i} + 1)^2}$$

\[ 
\left( \frac{\partial^2 Q}{\partial^2 w} \right)_{F+1, F+1} =\frac{1}{L} C_{F+1, L} \cdot D_{L, F+1}
\]

$$C_{j, i} = \frac{x_{i, j}}{e^{\langle\,w,x_i\rangle \cdot y_i} + 1}$$

$$D_{i, k} = \frac{x_{i, k} \cdot e^{\langle\,w,x_i\rangle \cdot y_i}}{e^{\langle\,w,x_i\rangle \cdot y_i} + 1} = \frac{x_{i, k} }{1 + e^{-\langle\,w,x_i\rangle \cdot y_i} } $$

$$\frac{\partial^2 Q^{l_2}}{\partial w_j \partial w_k} = \frac{\partial^2 Q}{\partial w_j \partial w_k} + \lambda \frac{\partial w_j}{\partial w_k}$$

\[\frac{\partial w_j}{\partial w_k} = \begin{cases} 
      0 & j \neq k\\
     1 & j = k \\
   \end{cases}
\]


$$\frac{\partial^2 Q^{l_2}}{\partial^2 w} = \frac{\partial^2 Q}{\partial^2 w} + \lambda I_{F+1}$$


\end{document}